theories/Syntax/RealResource.v
@@ -8,11 +8,11 @@ Import Streams.
 
 Definition t : Type := (Stream Λ * Stream Λ).
 
-Definition next (rr : t) : Λ * t := 
-  let (inp,out) := rr in (hd inp, (tl inp,out)).
+Definition next (rr : t) : Λ := 
+  let (inp,_) := rr in hd inp.
 
 Definition put (v : Λ) (rr : t) : t :=
-  let (inp,out) := rr in (inp,Cons v out).
+  let (inp,out) := rr in (tl inp,Cons v out).
 
 Definition put_opt (v : option Λ) (rr : t) : t :=
   match v with
@@ -24,6 +24,27 @@ Definition halts (rr : t) :=
   ForAll (fun st => halts (Streams.hd st)) (fst rr) /\
   ForAll (fun st => halts (Streams.hd st)) (snd rr).
 
+Lemma halts_next t : 
+  halts t -> Evaluation.halts (next t).
+Proof.
+  intros. destruct t; simpl; destruct H; simpl in *.
+  destruct s; simpl in *; inversion H; now simpl in *.
+Qed.
+
+Lemma halts_put t v :
+  halts t -> Evaluation.halts v -> halts (put v t).
+Proof.
+  intros; unfold put; destruct t; destruct H; split; simpl in *.
+  - inversion H; auto.
+  - split; simpl; auto.
+Qed. 
+
+Lemma halts_put_opt t v :
+  halts t -> match v with Some v => Evaluation.halts v | _ => True end -> halts (put_opt v t).
+Proof.
+  intros. destruct v; auto. unfold put_opt; now apply halts_put.
+Qed. 
+
 End RealResource.
 
 
@@ -34,12 +55,34 @@ Import List.
 
 Definition t : Type := list RealResource.t.
 
-Definition nexts (fl : t) : list Λ * t :=
-  split (map RealResource.next fl).
+Definition nexts (fl : t) : list Λ := map RealResource.next fl.
 
 Definition puts (vl : list (option Λ)) (fl : t) : t :=
   map (fun vf => RealResource.put_opt (fst vf) (snd vf)) (combine vl fl).
 
 Definition halts := List.Forall RealResource.halts.
+
+Lemma halts_nexts t : 
+  halts t -> List.Forall Evaluation.halts (nexts t).  
+Proof.
+  unfold halts; intros; induction H; simpl; auto.
+  apply List.Forall_cons_iff; split; auto. now apply RealResource.halts_next.
+Qed.
+
+Lemma halts_puts t vl :
+  halts t -> 
+  List.Forall (fun v => match v with Some v => Evaluation.halts v | _ => True end) vl ->
+  halts (puts vl t).
+Proof.
+  revert vl; induction t; intros; simpl in *.
+  - unfold puts, combine; destruct vl; simpl; auto.
+  - destruct vl.
+    -- unfold puts; simpl; unfold halts; auto.
+    -- unfold puts; simpl; unfold halts in *. apply Forall_cons_iff; split.
+       + rewrite Forall_cons_iff in *; destruct H,H0.
+         apply RealResource.halts_put_opt; auto; destruct o; auto.
+       + rewrite Forall_cons_iff in *; destruct H,H0.
+         apply IHt; auto.
+Qed.
 
 End RealResources.
