theories/Temporal.v
@@ -12,16 +12,16 @@ rsf's semantics are divided in three sub semantics:
 *)
 
 Module RE := REnvironment.
-Reserved Notation "'Instₜₜ(' Re , Rf )" (at level 50).
+Reserved Notation "'Wfₜₜ(' Re , Rf )" (at level 50).
 
 (** *** Definition *)
 
 Inductive temporal : RealResources.t -> RealResources.t -> Λ -> Λ -> Prop :=
- TT_instant : forall Vin Vout (R R' : RealResources.t) (P P' : Λ),
+ TT_instant : forall Vin Vout _tv (R R' : RealResources.t) (P P' : Λ),
 
-                    (Vin = RE.embeds (fst (RealResources.nexts R)))%re ->
-                    ⪡ Vin ; unit ; P ⪢ ⭆ ⪡ Vout ; unit ; P' ⪢ ->
-                    R' = RealResources.puts (RE.extracts Vout) (snd (RealResources.nexts R)) -> 
+                    (Vin = RE.embeds (RealResources.nexts R))%re ->
+                    ⪡ Vin ; unit ; P ⪢ ⭆ ⪡ Vout ; _tv ; P' ⪢ ->
+                    R' = RealResources.puts (RE.extracts Vout) R -> 
                     
                     temporal R R' P P'.
 
@@ -41,23 +41,43 @@ Notation "'⟦' R ';' P '⟧' '⟾⋆' '⟦' R1 ';' P1 '⟧'" := (multi_temporal
                                                          P custom rsf, P1 custom rsf, 
                                                         no associativity).
 
-Inductive instantiation_temp : ℜ -> RealResources.t -> Prop :=
-  | itTT_empty  : forall (Re : ℜ) (Fl : RealResources.t), 
-                     isEmptyᵣᵪ(Re) -> Instₜₜ(Re,nil)
+Inductive wf_env_TT : ℜ -> RealResources.t -> Prop :=
+  | wfTT_empty  : forall (Re : ℜ) (Fl : RealResources.t), 
+                     isEmptyᵣᵪ(Re) -> Wfₜₜ(Re,nil)
 
-  | itTT_init   : forall (Re Re' : ℜ) (Fl : RealResources.t) (τ τ' : Τ) (r : RealResource.t),
-      Instₜₜ(Re,Fl) ->
+  | wfTT_init   : forall (Re Re' : ℜ) (Fl : RealResources.t) (τ τ' : Τ) (r : RealResource.t),
+      Wfₜₜ(Re,Fl) ->
       Addᵣᵪ (newᵣᵪ(Re)) (τ,τ') Re Re' ->
-      Streams.ForAll (fun v => ∅ᵥᵪ ⋅ Re ⊫ {Streams.hd v} ∈ τ) (fst r) -> 
-      Streams.ForAll (fun v => ∅ᵥᵪ ⋅ Re ⊫ {Streams.hd v} ∈ τ') (snd r) -> 
-      Instₜₜ(Re',Fl ++ (r :: nil))
-(*
-  | itfT_update : forall (Re : ℜ) (V V' : 𝓥) r (τ τ' : Τ) (v : Λ),
-                    Instᵣₜ(Re,V) -> Re ⌈r ⩦ (τ,τ')⌉ᵣᵪ -> 
-                    r ∈ᵣᵦ V -> Addᵣᵦ r ((⩽ … v ⩾)) V V' -> 
-                    ∅ᵥᵪ ⋅ Re ⊫ v ∈ τ -> Instᵣₜ(Re,V')
-*)
-where "'Instₜₜ(' Re , Fl )" := (instantiation_temp Re Fl).
+      Streams.ForAll (fun v => ∅ᵥᵪ ⋅ Re ⊫ {Streams.hd v} ∈ τ') (fst r) -> 
+      Streams.ForAll (fun v => ∅ᵥᵪ ⋅ Re ⊫ {Streams.hd v} ∈ τ) (snd r) -> 
+      Wfₜₜ(Re',Fl ++ (r :: nil))
+
+  | wfTT_update : forall (Re : ℜ) (V : 𝓥) Rf,
+                    Wfᵣₜ(Re,V) -> 
+                    Wfₜₜ(Re,Rf) ->
+                    Wfₜₜ(Re,RealResources.puts (RE.extracts V) Rf)
+where "'Wfₜₜ(' Re , Fl )" := (wf_env_TT Re Fl).
+
+Lemma wf_env_TT_to_fT Re Fl : 
+  Wfₜₜ(Re,Fl) -> Wfᵣₜ(Re,RE.embeds (RealResources.nexts Fl)).
+Proof.
+  intro inst; induction inst; simpl.
+  - unfold RE.embeds; simpl; apply wfFT_empty; auto.
+    apply RE.OP.P.empty_1.
+  - destruct r; simpl in *. unfold RealResources.nexts.
+    rewrite map_app; simpl. unfold RE.embeds.
+    unfold RE.embeds_gen; rewrite <- fold_left_rev_right. 
+    fold RE.embeds_func_revert. rewrite rev_unit; simpl.
+    rewrite fold_left_rev_right. unfold RE.embeds_func_revert.
+    replace (fold_left (fun (x : RE.t) (y : Λ) => RE.embeds_func x y) (map RealResource.next Fl) (∅ᵣᵦ))
+    with (RE.embeds (RealResources.nexts Fl)); auto.
+    unfold RE.embeds_func.
+    
+    destruct s; simpl in *. inversion H0; simpl in *.
+    eapply wfFT_init with (v := λ); eauto.
+    unfold RE.OP.P.Add; reflexivity.
+  - admit.
+Admitted.
 
 (** *** Initialization *)
 
@@ -71,7 +91,7 @@ Qed.
 Lemma resource_used_init_unused : forall Re t α β R l V,
   ∅ᵥᵪ ⋅ Re ⊫ t ∈ (α ⟿ β ∣ R) ->
   halts t ->
-  Instᵣₜ(Re,V) ->
+  Wfᵣₜ(Re,V) ->
   (V = (RE.embeds l))%re ->
   
   (forall r, (r ∈ R)%rs -> RE.unused r V).
@@ -79,63 +99,87 @@ Proof.
   intros. destruct H0 as [t' [HmeT Hvt']].
   apply multi_preserves_typing with (t' := t') in H; auto.
   apply typing_Re_R with (r := r) in H; auto.
-  apply instantiation_in with (V := V) in H; auto.
+  apply wf_env_fT_in with (V := V) in H; auto.
   rewrite H2 in *. destruct H; apply RE.OP.P.find_1 in H.
   apply initialization_unused in H as H'; destruct x; inversion H'.
   exists λ. now rewrite H2.
 Qed. 
 
+
 (** *** Proof of typing preservation through the temporal transition *)
 Theorem temporal_preserves_typing (Re : ℜ) Rf Rf' (P P' : Λ) (R : resources) :
 
+    (* (1) *) halts P -> (* (2) *) RealResources.halts Rf -> (* (3) *) all_arrow_halting ->
+
     (* (1) *) ∅ᵥᵪ ⋅ Re ⊫ P ∈ (𝟙 ⟿ 𝟙 ∣ R) ->
     (* (3) *) ⟦ Rf ; P ⟧ ⟾ ⟦ Rf' ; P' ⟧ ->
-              Instₜₜ(Re,Rf) ->
+              Wfₜₜ(Re,Rf) ->
 
-  (*---------------------------------------------------------------------------------------------*)
-      ∅ᵥᵪ ⋅ Re ⊫ P' ∈ (𝟙 ⟿ 𝟙 ∣ R) /\ Instₜₜ(Re,Rf').
+  (*----------------------------------------------------*)
+      ∅ᵥᵪ ⋅ Re ⊫ P' ∈ (𝟙 ⟿ 𝟙 ∣ R) /\ Wfₜₜ(Re,Rf') /\ 
+       (* (7) *) halts P' /\ (* (8) *) RealResources.halts Rf'.
 Proof.
-  intros HwP HTT Hinst; inversion HTT; subst. 
-  (*
-  destruct (RealResources.nexts Rf) as [sample tail]; simpl in *.
+  intros HltP HltRf HlAll HwP HTT Hinst; inversion HTT; subst.
+  apply wf_env_TT_to_fT in Hinst as Hinst'.
   eapply functional_preserves_typing in H0; eauto.
-  - split; destruct H0 as [_ [_ [HinstV [_ [_ HwP']]]]].
-    -- assumption.
-    -- 
-  - now constructor.
+  - repeat split; destruct H0 as [_ [_ [HinstV [_ [_ [HwP' [HltP' [_ HltVout]]]]]]]]; auto.
+    -- constructor; auto.
+    -- apply RealResources.halts_puts; auto. now apply RE.halts_extract.
+  - exists <[unit]>; split; auto.
+  - apply REnvironment.halts_nexts in HltRf. unfold RE.halts; intros. rewrite H in *.
+    eapply HltRf; eauto. 
   - now rewrite H.
-Qed.*)
-Admitted.
+Qed.
 
-(*
 (** *** Proof of typing preservation through multi temporal transitions *)
 Theorem multi_temporal_preserves_typing (Re : ℜ) Rf Rf' (P P' : Λ) (R : resources) :
+    (* (1) *) halts P -> (* (2) *) RealResources.halts Rf -> (* (3) *) all_arrow_halting ->
 
     (* (1) *) ∅ᵥᵪ ⋅ Re ⊫ P ∈ (𝟙 ⟿ 𝟙 ∣ R) ->
     (* (3) *) ⟦ Rf ; P ⟧ ⟾⋆ ⟦ Rf' ; P' ⟧ ->
-              Instᵣₜ(Re,RE.embeds (fst (RealResources.nexts Rf))) ->
+              Wfₜₜ(Re,Rf) ->
 
-  (*---------------------------------------------------------------------------------------------*)
-      ∅ᵥᵪ ⋅ Re ⊫ P' ∈ (𝟙 ⟿ 𝟙 ∣ R).
+  (*----------------------------------------------------*)
+      ∅ᵥᵪ ⋅ Re ⊫ P' ∈ (𝟙 ⟿ 𝟙 ∣ R) /\ Wfₜₜ(Re,Rf') /\ 
+       (* (7) *) halts P' /\ (* (8) *) RealResources.halts Rf'.
 Proof.
-  intros HwP HTT Hinst; induction HTT; subst.
-  eapply temporal_preserves_typing in H; eauto; apply IHHTT; auto.  
-  destruct (RealResources.nexts Rf) as [sample tail]; simpl in *.
-  eapply functional_preserves_typing in H0; eauto.
-  - now destruct H0 as [_ [_ [_ [_ [_ HwP']]]]].
-  - now constructor.
-  - now rewrite H.
+  intros HltP HltRf HAll HwP HTT; induction HTT; subst; intros.
+  eapply temporal_preserves_typing in H as [HwP' [HWf [HltP' HlR0]]]; eauto.
 Qed.
-*)
+
 
 Theorem progress_of_temporal (Re : ℜ) (Rf : RealResources.t) (P : Λ) (R : resources) :
 
   (* (1) *) halts P -> (* (2) *) RealResources.halts Rf -> (* (3) *) all_arrow_halting ->
 
-  (* (4) *) ∅ᵥᵪ ⋅ Re ⊫ P ∈ (𝟙 ⟿ 𝟙 ∣ R) -> (* (5) *) Instₜₜ(Re,Rf) ->
+  (* (4) *) ∅ᵥᵪ ⋅ Re ⊫ P ∈ (𝟙 ⟿ 𝟙 ∣ R) -> (* (5) *) Wfₜₜ(Re,Rf) ->
   
   (*-------------------------------------------------------------------------------------------------*)
-    exists Rf' P',  (* (6) *) ⟦ Rf ; P ⟧ ⟾⋆ ⟦ Rf' ; P' ⟧ /\ 
-                    (* (7) *) halts P' /\ (* (8) *) RealResources.halts Rf.
-Proof. 
-Admitted.
+    exists Rf' P',  (* (6) *) ⟦ Rf ; P ⟧ ⟾ ⟦ Rf' ; P' ⟧ /\ 
+                    (* (7) *) halts P' /\ (* (8) *) RealResources.halts Rf'.
+Proof.
+  intros HltP HltRf HlAll HwP Hinst. 
+  assert (HwU : ∅ᵥᵪ ⋅ Re ⊫ unit ∈ 𝟙). { now constructor. }
+  remember (RE.embeds (RealResources.nexts Rf)) as Vin.
+
+  eapply progress_of_functional with (V := Vin) in HwU; eauto.
+  - destruct HwU as [Vout [tv' [P' [HfT [HltP' [Hltv' HltVout]]]]]].
+    exists (RealResources.puts (RE.extracts Vout) Rf); exists P'; repeat split; auto.
+    -- econstructor; eauto; subst; reflexivity.
+    -- apply RealResources.halts_puts; auto. now apply RE.halts_extract.
+  - exists <[unit]>; split; auto.
+  - apply REnvironment.halts_nexts in HltRf. unfold RE.halts; intros. rewrite HeqVin in *.
+    eapply HltRf; eauto. 
+  - subst. now apply wf_env_TT_to_fT.
+  - apply wf_env_TT_to_fT in Hinst.
+    destruct HltP as [P' [HmeT HltP']].
+    eapply multi_preserves_typing in HwP; eauto.
+    intros. apply typing_Re_R with (r := r) in HwP; auto.
+    rewrite wf_env_fT_in in HwP; eauto.
+    unfold RE.unused. 
+    assert (RE.For_all (fun _ v => Cell.unused v) (RE.embeds (RealResources.nexts Rf))).
+    { apply initialization_unused. }
+    unfold RE.For_all in *. destruct HwP. apply RE.OP.P.find_1 in H1.
+    apply H0 in H1 as Hunsd. destruct x; inversion Hunsd. exists λ.
+    now rewrite HeqVin.
+Qed.
